code/ecdsa/Hacl.Impl.P256.LowLevel.fst
@@ -124,7 +124,7 @@ let add_dep_prime_p256 x t result =
 
   cc
 
-
+inline_for_extraction noextract
 val mul64: x: uint64 -> y: uint64 -> result: lbuffer uint64 (size 1) -> temp: lbuffer uint64 (size 1) ->
   Stack unit (requires fun h -> live h result /\ live h temp /\ disjoint result temp)
   (ensures fun h0 _ h1 -> modifies (loc result |+| loc temp) h0 h1 /\ (
@@ -157,7 +157,6 @@ let mult64_c x u cin result temp =
   add_carry_u64 cin l h result
 
 
-inline_for_extraction noextract
 val shortened_mul_prime256: b: uint64 -> result: widefelem P256 -> Stack unit
   (requires fun h -> live h result /\ wide_as_nat P256 h result < pow2 (64 * 5))
   (ensures fun h0 _ h1 -> modifies (loc result) h0 h1 /\ wide_as_nat P256 h1 result < pow2 (64 * 5) /\
